# Pattern exemplification core concepts schema
# This document defines and provides the vocabulary to talk about relations between a design pattern and an example of its instantiation.
# Many aspects of design patterns and exemplars/annotations can be descibed using existing vocabularies eg dublin core - and where suitable we prefer to use these terms directly rather than invent 
# new subclasses of them here
# This document therefore only covers the intrinsic core pattern emeplification elements, and is intended to be extsnsible and evolvable.


@prefix : <http://purl.org/NET/exemplr#> .
@prefix lp: <http://purl.org/NET/labpatterns#> .
@prefix dcterms: <http://purl.org/dc/terms/> .
@prefix foaf: <http://xmlns.com/foaf/0.1/> .
@prefix owl: <http://www.w3.org/2002/07/owl#> .
@prefix rdf: <http://www.w3.org/1999/02/22-rdf-syntax-ns#> .
@prefix rdfs: <http://www.w3.org/2000/01/rdf-schema#> .
@prefix xsd: <http://www.w3.org/2001/XMLSchema#> .




###################################
# General Schema Info
###################################

:
	rdf:type owl:Ontology ;
	dcterms:title "Schema to describe Design Pattern Exemplifcations"@en ;
	rdfs:label "Design Pattern Exemplar Schema"^^xsd:string ;
	rdfs:comment "A simple schema for describing annotations that capture design pattern examples."@en ;
	foaf:maker :cam ;
	dcterms:created "2015-05-19"^^xsd:date ;
	dcterms:license <http://creativecommons.org/licenses/by/4.0#id> .



:cam rdf:type foaf:Person ;
	<http://vivoweb.org/ontology/core#orcidId> <http://orcid.org/0000-0002-9836-3824> ;
	foaf:name "Cameron McLean" ;
	foaf:homepage <http://cameronmclean.github.io> .



###################
# Classes
###################

:Exemplar a owl:Class ;
	rdfs:label "Exemplar"@en ;
	rdfs:comment "A an Exemplar is a graph structure that ties together a design pattern with an instance of its application, exemplifying how the forces are dealt with in a concrete design."@en ;
	rdfs:isDefinedBy : .


##############################
# ObjectProperties
##############################


:concernsForce rdf:type owl:ObjectProperty ;
	rdfs:label "concerns Force"@en ;
	rdfs:comment "Names the pattern force(s) the specific exemplar highlights examples of."@en ;
	rdfs:domain :Exemplar ;
	rdfs:range lp:Force ;
	rdfs:isDefinedBy : .


:concernsPattern rdf:type owl:ObjectProperty ;
	rdfs:label "concerns Pattern"@en ;
	rdfs:comment "Names the pattern which the specific exemplar concerns."@en ;
	rdfs:domain :Exemplar ;
	rdfs:range lp:Pattern ;
	rdfs:isDefinedBy : .


:hasTargetURL rdf:type owl:ObjectProperty ;
	rdfs:label "has target"@en ;
	rdfs:comment "The protocol resource (instance) the exemplar points to."@en ;
	rdfs:domain :Exemplar ;
	rdfs:isDefinedBy : .


:creatorORCID rdf:type owl:DataTypeProperty ;
	rdfs:label "creator ORCID"@en ;
	rdfs:comment "ORCID resource that identifies the person who created the exemplar/annotation."@en ;
	rdfs:isDefinedBy : .


###################################
#  Datatype Properties
###################################



:hasTargetDetail rdf:type owl:DatatypeProperty ;
	rdfs:label "has detail"@en ;
	rdfs:comment "The specific text fragment from the protocol that constitutes the exemplar."@en ;
	rdfs:domain :Exemplar ;
	rdfs:range xsd:string ;
	rdfs:isDefinedBy : .

:hasTargetTitle rdf:type owl:DatatypeProperty ;
	rdfs:label "has title"@en ;
	rdfs:comment "The title of the protocol web resource that the exemplar refers to."@en ;
	rdfs:domain :Exemplar ;
	rdfs:range xsd:string ;
	rdfs:isDefinedBy : .

:exemplifiedBy rdf:type owl:DatatypeProperty ;
	rdfs:label "exemplified by"@en ;
	rdfs:comment "Relates a pattern force to a literal string describing an instance of how the force was dealt with."@en ;
	rdfs:domain lp:Force ;
	rdfs:range xsd:string ;
	rdfs:isDefinedBy : .

:hasComment rdf:type owl:DatatypeProperty ;
	rdfs:label "has comment"@en ;
	rdfs:comment "Describes additional details relevant to how the target exemplifies the pattern and forces"@en ;
	rdfs:domain :Exemplar ;
	rdfs:range xsd:string ;
	rdfs:isDefinedBy : .
